Compiler/Test.v
@@ -24,12 +24,14 @@ Definition dep_cart_prod{X}{Y : X -> Type}(xs : list X)(ys : forall x, list (Y x
 Section Params.
 
 Definition num := 5.
-Definition idxNum := 20.
-Definition Data := Bit 32.
-Definition init_val : word 32 := (NToWord _ 323711244).
+Definition idxNum := 120.
+Definition Xlen := 32.
+Definition Data := Bit Xlen.
+Definition Counter := Bit 2.
+Definition init_val : word Xlen := Xlen 'h"abc123".
 
 (* mask = {true; false; false; false; true} *)
-Definition mask_func : Fin.t num -> bool := fun (i : Fin.t num) =>
+Definition mask_func1 : Fin.t num -> bool := fun (i : Fin.t num) =>
   match i with
   | F1 _ => true
   | FS _ (F1 _) => false
@@ -38,20 +40,23 @@ Definition mask_func : Fin.t num -> bool := fun (i : Fin.t num) =>
   | _ => true
   end.
 
-Definition mask_func_inv : Fin.t num -> bool := fun i => negb (mask_func i).
+Definition mask_func2 : Fin.t num -> bool := fun i => negb (mask_func1 i).
 
-Definition mask : ConstT (Array num Bool) := ConstArray mask_func.
-Definition mask_inv : ConstT (Array num Bool) := ConstArray mask_func_inv.
+Definition mask1 : ConstT (Array num Bool) := ConstArray mask_func1.
+Definition mask2 : ConstT (Array num Bool) := ConstArray mask_func2.
 
 Definition write_index := 4.
 Definition read_under_index := 2.
 Definition read_over_index := 6.
 Definition read_disjoint_index := 12.
 
-Definition write_val_1 : word 32 := NToWord _ 512345234.
-Definition write_val_2 : word 32 := NToWord _ 423413.
+Definition write_val_1 : word Xlen := Xlen 'h"def345".
+Definition write_val_2 : word Xlen := Xlen 'h"bdf678".
 
 (* reality check lemmas *)
+
+(* good read/write indices*)
+
 Lemma read_under_bounds : read_under_index < write_index < read_under_index + num.
 Proof.
   cbv delta; lia.
@@ -67,25 +72,49 @@ Proof.
   cbv delta; lia.
 Qed.
 
-Lemma mask_under_true : exists (i : Fin.t num), mask_func i = true /\ f2n i < num - (write_index - read_under_index).
+(*good masks*)
+
+Lemma mask1_under_true : exists (i : Fin.t num), mask_func1 i = true /\ f2n i < num - (write_index - read_under_index).
 Proof.
   exists F1; simpl; auto.
 Qed.
 
-Lemma mask_under_false : exists (i : Fin.t num), mask_func i = false /\ f2n i < num - (write_index - read_under_index).
+Lemma mask1_under_false : exists (i : Fin.t num), mask_func1 i = false /\ f2n i < num - (write_index - read_under_index).
 Proof.
   exists (FS F1); simpl; auto.
 Qed.
 
-Lemma mask_over_true : exists (i : Fin.t num), mask_func i = true /\ f2n i > (read_over_index - write_index).
+Lemma mask1_over_true : exists (i : Fin.t num), mask_func1 i = true /\ f2n i > (read_over_index - write_index).
 Proof.
   exists (FS (FS (FS (FS F1)))); unfold f2n; simpl; auto.
 Qed.
 
-Lemma mask_over_false : exists (i : Fin.t num), mask_func i = false /\ f2n i > (read_over_index - write_index).
+Lemma mask1_over_false : exists (i : Fin.t num), mask_func1 i = false /\ f2n i > (read_over_index - write_index).
 Proof.
   exists (FS (FS (FS F1))); unfold f2n; simpl; auto.
 Qed.
+
+Lemma mask2_under_true : exists (i : Fin.t num), mask_func2 i = true /\ f2n i < num - (write_index - read_under_index).
+Proof.
+  exists (FS F1); simpl; auto.
+Qed.
+
+Lemma mask2_under_false : exists (i : Fin.t num), mask_func2 i = false /\ f2n i < num - (write_index - read_under_index).
+Proof.
+  exists F1; simpl; auto.
+Qed.
+
+Lemma mask2_over_true : exists (i : Fin.t num), mask_func2 i = true /\ f2n i > (read_over_index - write_index).
+Proof.
+  exists (FS (FS (FS F1))); unfold f2n; simpl; auto.
+Qed.
+
+Lemma mask2_over_false : exists (i : Fin.t num), mask_func2 i = false /\ f2n i > (read_over_index - write_index).
+Proof.
+  exists (FS (FS (FS (FS F1)))); unfold f2n; simpl; auto.
+Qed.
+
+(* good values *)
 
 Lemma init_write1_neq : weqb init_val write_val_1 = false.
 Proof.
@@ -263,10 +292,10 @@ Variable tup : FileTuple.
 Definition all_init : ConstT (Array num Data) :=
   ConstArray (fun _ => init_val).
 
-Definition expected_read_under(val : word 32) : ConstT (Array num Data) :=
+Definition expected_read_under(val : word Xlen) : ConstT (Array num Data) :=
     ConstArray (fun i => if f2n i <? write_index - read_under_index then init_val else val).
 
-Definition expected_read_over(val : word 32) : ConstT (Array num Data) :=
+Definition expected_read_over(val : word Xlen) : ConstT (Array num Data) :=
     ConstArray (fun i => if f2n i <? num - (read_over_index - write_index) then val else init_val).
 
 (*translations*)
@@ -291,43 +320,45 @@ Proof.
   lia.
 Defined.
 
-Definition expected_read_under_masked(mask_val non_mask_val : word 32)(mf : Fin.t num -> bool) : ConstT (Array num Data) :=
+Definition expected_read_under_masked(mask_val non_mask_val : word Xlen)(mf nmf : Fin.t num -> bool) : ConstT (Array num Data) :=
   ConstArray (fun i => if f2n i <? write_index - read_under_index then init_val else
-    if mf (read_under_Fin_to_write_Fin i) then mask_val else non_mask_val).
+    if mf (read_under_Fin_to_write_Fin i) then mask_val else 
+    if nmf (read_under_Fin_to_write_Fin i) then non_mask_val else init_val).
 
-Definition expected_read_over_masked(mask_val non_mask_val : word 32)(mf : Fin.t num -> bool) : ConstT (Array num Data) :=
+Definition expected_read_over_masked(mask_val non_mask_val : word Xlen)(mf nmf : Fin.t num -> bool) : ConstT (Array num Data) :=
   ConstArray (fun i => match Compare_dec.le_lt_dec (num - (read_over_index - write_index)) (f2n i) with
                        | left _ => init_val
-                       | right pf => if mf (read_over_Fin_to_write_Fin i pf) then mask_val else non_mask_val
+                       | right pf => if mf (read_over_Fin_to_write_Fin i pf) then mask_val else
+                                     if nmf (read_over_Fin_to_write_Fin i pf) then non_mask_val else init_val
                        end).
 
-Definition expected_read_ot_mt(curr_val old_val : word 32)(mf : Fin.t num -> bool)(ot : OverlapType)(mt : MaskType) :=
+Definition expected_read_ot_mt(write_val old_val : word Xlen)(wmf omf : Fin.t num -> bool)(ot : OverlapType)(mt : MaskType) :=
   match ot,mt with
-  | Over,IsWrMask => expected_read_over_masked curr_val old_val mf
-  | Over,NotIsWrMask => expected_read_over curr_val
-  | Under,IsWrMask => expected_read_under_masked curr_val old_val mf
-  | Under,NotIsWrMask => expected_read_under curr_val
+  | Over,IsWrMask => expected_read_over_masked write_val old_val wmf omf
+  | Over,NotIsWrMask => expected_read_over write_val
+  | Under,IsWrMask => expected_read_under_masked write_val old_val wmf omf
+  | Under,NotIsWrMask => expected_read_under write_val
   | Disjoint,_ => all_init
   end.
 
 Definition expected_read_val_first_cycle : ConstT (Array num Data) :=
   let '(p,ot,mt) := tup in
     match p with
-    | existT AsyncF WriteRead => expected_read_ot_mt write_val_1 init_val mask_func ot mt
+    | existT AsyncF WriteRead => expected_read_ot_mt write_val_1 init_val mask_func1 mask_func2 ot mt
     | existT AsyncF ReadWrite => all_init
-    | _ => all_init (* don't care about Syncs during first cycle *)
+    | _ => getDefaultConst (Array num Data)
     end.
 
 Definition expected_read_val_second_cycle : ConstT (Array num Data) :=
   let '(p,ot,mt) := tup in
     match p with
-    | existT AsyncF WriteRead => expected_read_ot_mt write_val_2 write_val_1 mask_func_inv ot mt
-    | existT AsyncF ReadWrite => expected_read_ot_mt write_val_1 init_val mask_func ot mt
-    | existT SyncIsAddr WriteFirst => expected_read_ot_mt write_val_2 write_val_1 mask_func_inv ot mt
-    | existT SyncIsAddr WriteSecond => expected_read_ot_mt write_val_1 init_val mask_func ot mt
-    | existT SyncIsAddr WriteThird => expected_read_ot_mt write_val_1 init_val mask_func ot mt
-    | existT SyncNotIsAddr WriteFirst => expected_read_ot_mt write_val_1 init_val mask_func ot mt
-    | existT SyncNotIsAddr WriteSecond => expected_read_ot_mt write_val_1 init_val mask_func ot mt
+    | existT AsyncF WriteRead => expected_read_ot_mt write_val_2 write_val_1 mask_func2 mask_func1 ot mt
+    | existT AsyncF ReadWrite => expected_read_ot_mt write_val_1 init_val mask_func1 (fun _ => true) ot mt
+    | existT SyncIsAddr WriteFirst => expected_read_ot_mt write_val_2 write_val_1 mask_func2 mask_func1 ot mt
+    | existT SyncIsAddr WriteSecond => expected_read_ot_mt write_val_1 init_val mask_func1 (fun _ => true) ot mt
+    | existT SyncIsAddr WriteThird => expected_read_ot_mt write_val_1 init_val mask_func1 (fun _ => true) ot mt
+    | existT SyncNotIsAddr WriteFirst => expected_read_ot_mt write_val_1 init_val mask_func1 (fun _ => true) ot mt
+    | existT SyncNotIsAddr WriteSecond => expected_read_ot_mt write_val_1 init_val mask_func1 (fun _ => true) ot mt
     | existT SyncNotIsAddr WriteThird => all_init
     end.
 
@@ -336,15 +367,15 @@ Definition make_write : RuleT :=
   match mt with
   | IsWrMask => (("rule_" ++ write_name tup)%string,
       fun ty : (Kind -> Type) =>
-        Read c : Bool <- "counter";
-        LET write_val <- ITE (#c) $$write_val_2 $$write_val_1;
-        LET mask' <- ITE (#c) $$mask_inv $$mask;
-        Call (write_name tup)(@createWriteRqMask ty idxNum num Data ($write_index) (BuildArray (fun _ => #write_val)) #mask' : _); Retv
+        Read c : Counter <- "counter";
+        LET write_val <- ITE (#c == $1) $$write_val_2 $$write_val_1;
+        LET mask <- ITE (#c == $1) $$mask2 $$mask1;
+        Call (write_name tup)(@createWriteRqMask ty idxNum num Data ($write_index) (BuildArray (fun _ => #write_val)) #mask : _); Retv
       )
   | NotIsWrMask => (("rule_" ++ write_name tup)%string,
       fun ty : (Kind -> Type) =>
-        Read c : Bool <- "counter";
-        LET write_val <- ITE (#c) $$write_val_2 $$write_val_1;
+        Read c : Counter <- "counter";
+        LET write_val <- ITE (#c == $1) $$write_val_2 $$write_val_1;
         Call (write_name tup)(@createWriteRq ty idxNum num Data ($write_index) (BuildArray (fun _ => #write_val)) : _); Retv
       )
   end.
@@ -361,6 +392,12 @@ Definition print_comparison{ty k}(val exp_val : Expr ty (SyntaxKind k)) : list (
    DispString _ "\n\n"
   ].
 
+Definition print_read{ty}(read_idx : Expr ty (SyntaxKind (Bit (Nat.log2_up idxNum)))) : list (SysT ty) :=
+  [DispString _ "Read Index: ";
+   DispHex read_idx;
+   DispString _ "\n\n"
+  ].
+
 Definition make_read : RuleT :=
   let '((existT ft sch),ot,mt) := tup in
   let read_index := match ot with
@@ -371,9 +408,9 @@ Definition make_read : RuleT :=
   (("rule_" ++ read_name tup)%string,
   fun (ty : Kind -> Type) => 
     Call val : Array num Data <- (read_name tup)($read_index : Bit (Nat.log2_up idxNum));
-    Read c : Bool <- "counter";
-    LET exp_val : Array num Data <- ITE #c $$expected_read_val_second_cycle $$expected_read_val_first_cycle;
-    System (print_comparison #val #exp_val);
+    Read c : Counter <- "counter";
+    LET exp_val : Array num Data <- ITE (#c == $1) $$expected_read_val_second_cycle $$expected_read_val_first_cycle;
+    System ([DispString _  ("rule_" ++ read_name tup ++ ":\n")%string] ++ print_read ($read_index) ++ print_comparison #val #exp_val);
     Retv
   ).
 
@@ -385,16 +422,20 @@ Definition make_readReq : RuleT :=
                     | Disjoint => read_disjoint_index
                     end in
   (("rule_" ++ readReq_name tup)%string,
-  fun ty => Call (readReq_name tup)($read_index : Bit (Nat.log2_up idxNum)); Retv
+  fun ty => 
+      Call (readReq_name tup)($read_index : Bit (Nat.log2_up idxNum));
+      System ([DispString _  ("rule_" ++ readReq_name tup ++ ":\n")%string] ++ print_read ($read_index));
+      Retv
   ).
 
 Definition make_readResp : RuleT :=
   (("rule_" ++ readRes_name tup)%string,
   fun (ty : Kind -> Type) =>
     Call val : Array num Data <- (readRes_name tup)();
-    Read c : Bool <- "counter";
-    LET exp_val : Array num Data <- ITE #c $$expected_read_val_second_cycle $$expected_read_val_first_cycle;
-    System (print_comparison #val #exp_val);
+    Read c : Counter <- "counter";
+    LET exp_val : Array num Data <- ITE (#c == $1) $$expected_read_val_second_cycle $$expected_read_val_first_cycle;
+    System [DispString _  ("rule_" ++ readRes_name tup ++ ":\n")%string];
+    If (#c == $1) then (System (print_comparison #val #exp_val); Retv);
     Retv
   ).
 
@@ -425,38 +466,64 @@ Definition all_rf_rules : list RuleT :=
 (* write then read *)
 
 Definition write_reg_1 : RuleT :=
-  ("write_reg_1", fun ty : (Kind -> Type) =>
-      Read c : Bool <- "counter";
-      LET new_val : Data <- ITE (#c) $$write_val_2 $$write_val_1;
+  ("write_reg_WR", fun ty : (Kind -> Type) =>
+      Read c : Counter <- "counter";
+      LET new_val : Data <- ITE (#c == $1) $$write_val_2 $$write_val_1;
+      System ([DispString _  ("write_reg_WR: ")%string; DispHex #new_val; DispString _ "\n\n"]);
       Write "reg_1" <- #new_val;
       Retv
       ).
 
 Definition read_reg_1 : RuleT :=
-  ("read_reg_1", fun ty : (Kind -> Type) =>
-      Read c : Bool <- "counter";
+  ("read_reg_WR", fun ty : (Kind -> Type) =>
+      Read c : Counter <- "counter";
       Read val : Data <- "reg_1";
-      LET exp_val : Data <- ITE (#c) $$write_val_2 $$write_val_1;
-      System (print_comparison #val #exp_val);
+      LET exp_val : Data <- ITE (#c == $1) $$write_val_2 $$write_val_1;
+      System ([DispString _ "read_reg_WR:\n"] ++ print_comparison #val #exp_val);
       Retv
       ).
 
 (* read then write *)
 
 Definition read_reg_2 : RuleT :=
-  ("read_reg_2", fun ty : (Kind -> Type) =>
-      Read c : Bool <- "counter";
+  ("read_reg_RW", fun ty : (Kind -> Type) =>
+      Read c : Counter <- "counter";
       Read val : Data <- "reg_2";
-      LET exp_val : Data <- ITE (#c) $$write_val_1 $$init_val;
-      System (print_comparison #val #exp_val);
+      LET exp_val : Data <- ITE (#c == $1) $$write_val_1 $$init_val;
+      System ([DispString _ "read_reg_RW:\n"] ++ print_comparison #val #exp_val);
       Retv
       ).
 
 Definition write_reg_2 : RuleT :=
-  ("write_reg_2", fun ty : (Kind -> Type) =>
-      Read c : Bool <- "counter";
-      LET new_val : Data <- ITE (#c) $$write_val_2 $$write_val_1;
+  ("write_reg_RW", fun ty : (Kind -> Type) =>
+      Read c : Counter <- "counter";
+      LET new_val : Data <- ITE (#c == $1) $$write_val_2 $$write_val_1;
+      System ([DispString _  "write_reg_RW: "; DispHex #new_val; DispString _ "\n\n"]);
       Write "reg_2" <- #new_val;
+      Retv
+      ).
+
+Definition reg_3_rule_1 : RuleT :=
+  ("reg_3_write_1", fun ty : (Kind -> Type) =>
+      Write "reg_3" <- $$write_val_1;
+      Read val : Data <- "reg_3";
+      System ([DispString _ "reg_3_write_1:\n"] ++ print_comparison #val $$init_val);
+      Retv
+      ).
+
+Definition reg_3_rule_2 : RuleT :=
+  ("reg_3_write_2", fun ty : (Kind -> Type) =>
+      Write "reg_3" <- $$write_val_2;
+      Read val : Data <- "reg_3";
+      System ([DispString _ "reg_3_write_2:\n"] ++ print_comparison #val $$write_val_1);
+      Retv
+      ).
+
+Definition reg_3_rule_3 : RuleT :=
+  ("reg_3_init", fun ty : (Kind -> Type) =>
+      Write "reg_3" <- $$init_val;
+      Read val : Data <- "reg_3";
+      System ([DispString _ "reg_3_init:\n"] ++ print_comparison #val $$write_val_2);
       Retv
       ).
 
@@ -464,20 +531,22 @@ Definition write_reg_2 : RuleT :=
 
 Definition counter : RuleT :=
   ("counter", fun ty : (Kind -> Type) =>
-      Read x : Bool <- "counter";
-      If(#x) then
-        System [DispString _ "Finished."; Finish _]; Retv
+      Read c : Counter <- "counter";
+      System [DispString _ "End of cycle "; DispHex #c; DispString _ "\n"];
+      If(#c == $1) then
+        System [DispString _ "Finished.\n"; Finish _]; Retv
       else
-        Write "counter" <- $$true;
+        Write "counter" <- #c + $1;
         Retv;
       Retv).
 
-Definition all_reg_rules := [write_reg_1; read_reg_1; read_reg_2; write_reg_2].
+Definition all_reg_rules := [write_reg_1; read_reg_1; read_reg_2; write_reg_2; reg_3_rule_1; reg_3_rule_2; reg_3_rule_3].
 
 Definition testBaseMod := BaseMod [
   ("reg_1", (existT _ (SyntaxKind _) (Some (SyntaxConst init_val))));
   ("reg_2", (existT _ (SyntaxKind _) (Some (SyntaxConst init_val))));
-  ("counter", (existT _ (SyntaxKind _) (Some (SyntaxConst false))))
+  ("reg_3", (existT _ (SyntaxKind _) (Some (SyntaxConst init_val))));
+  ("counter", (existT _ (SyntaxKind (Counter)) (Some (SyntaxConst (getDefaultConst _)))))
   ]
  (all_reg_rules ++ all_rf_rules ++ [counter]) [].
 
